byteback-dummy/java8/src/main/java/byteback/dummy/condition/Boolean.java
@@ -1,0 +1,41 @@
+package byteback.dummy.condition;
+
+import static byteback.annotations.Operator.implies;
+import static byteback.annotations.Operator.not;
+
+import byteback.annotations.Contract.Condition;
+import byteback.annotations.Contract.Ensure;
+
+public class Boolean {
+
+  @Condition
+  public static boolean and_postcondition(boolean a, boolean b, boolean returns) {
+    return implies(a & b, returns);
+  }
+
+  @Condition
+  public static boolean or_postcondition(boolean a, boolean b, boolean returns) {
+    return implies(a | b, returns);
+  }
+
+  @Condition
+  public static boolean not_postcondition(boolean a, boolean returns) {
+    return implies(a, not(returns));
+  }
+
+  @Ensure("and_postcondition")
+	public static boolean shortCircuitingAnd(boolean a, boolean b) {
+		return a && b;
+	}
+
+  @Ensure("or_postcondition")
+	public static boolean shortCircuitingOr(boolean a, boolean b) {
+		return a || b;
+	}
+
+  @Ensure("not_postcondition")
+	public static boolean shortCircuitingNot(boolean a) {
+		return !a;
+	}
+
+}
